theories/grad_lang/dynamics/std.v
@@ -1,35 +1,7 @@
 From main.prelude Require Import base_lang labels imports autosubst.
-From main.grad_lang Require Export types.
+From main.grad_lang Require Export definition types definition.
 
-(* Important; we don't have labels anymore on destructors. *)
-(* Only on cast constructs *)
-
-Inductive expr :=
-  (* base values *)
-  | Lit (b : base_lit)
-  | Seq (e1 e2 : expr)
-  | If (e0 e1 e2 : expr)
-  | BinOp (binop : bin_op) (e1 e2 : expr)
-  (* functions *)
-  | Var (v : var)
-  | Lam (e : {bind 1 of expr})
-  | App (e1 e2 : expr)
-  (* sums *)
-  | InjL (e : expr)
-  | InjR (e : expr)
-  | Case (e0 : expr) (e1 e2 : {bind 1 of expr})
-  (* pairs *)
-  | Fst (e : expr)
-  | Snd (e : expr)
-  | Pair (e1 e2 : expr)
-  (* error *)
-  (* | Error (ℓ : label) *)
-  (* Easier if we have source type, then translation is easier *)
-  (* Also a proof of consistency? *)
-  (* | Cast (τ1 τ2 : type) (e : expr) *)
-  (* We want translation from surface to cast calculus to be definable without typing derivation... *)
-  | Cast (ℓ : label) (τ1 τ2 : type) (e : expr)
-  | Error (ℓ : label).
+(* this is a standard representation for the dynamics of our cast calculus *)
 
 Instance Ids_expr : Ids expr. derive. Defined.
 Instance Rename_expr : Rename expr. derive. Defined.
