theories/maps/dyn_embedding/definition.v
@@ -4,7 +4,7 @@ From main.grad_lang Require Import types definition typing.
 
 (* The dynamic embedding, of the dynamic language into the gradual one. *)
 
-Definition AscribeAn {ν : label} {Hν : NeverOccurs ν} := Ascribe ν.
+Definition CastAn {ν : label} {Hν : NeverOccurs ν} := Cast ν.
 
 Section dyn_emb.
 
@@ -16,24 +16,24 @@ Section dyn_emb.
   Fixpoint dyn_emb (e : dyn_lang.definition.expr) : grad_lang.definition.expr :=
     match e with
     | dyn_lang.definition.Lit b =>
-        AscribeAn (base_lit_type b) Unknown (Lit b)
+        CastAn (base_lit_type b) Unknown (Lit b)
     | dyn_lang.definition.Seq ℓ e1 e2 =>
         Seq
-           (Ascribe ℓ Unknown (Base Unit) (dyn_emb e1))
+           (Cast ℓ Unknown (Base Unit) (dyn_emb e1))
            (dyn_emb e2)
     | dyn_lang.definition.If ℓ e0 e1 e2 =>
         If
-           (Ascribe ℓ Unknown (Base Bool) (dyn_emb e0))
+           (Cast ℓ Unknown (Base Bool) (dyn_emb e0))
            (dyn_emb e1)
            (dyn_emb e2)
     | dyn_lang.definition.BinOp ℓ binop e1 e2 =>
         LetIn (Pair (dyn_emb e1) (dyn_emb e2)) (
           LetIn (Fst (Var 0)) (
             LetIn (Snd (Var 1)) (
-                  (Ascribe ℓ (binop_res_type binop) Unknown
+                  (Cast ℓ (binop_res_type binop) Unknown
                       (BinOp binop
-                          (Ascribe ℓ Unknown (Base Int) (Var 1))
-                          (Ascribe ℓ Unknown (Base Int) (Var 0)))
+                          (Cast ℓ Unknown (Base Int) (Var 1))
+                          (Cast ℓ Unknown (Base Int) (Var 0)))
                   )
                )
              )
@@ -41,23 +41,23 @@ Section dyn_emb.
     | dyn_lang.definition.Var v =>
         Var v
     | dyn_lang.definition.Lam e =>
-        AscribeAn (Bin Arrow Unknown Unknown) Unknown (Lam (dyn_emb e))
+        CastAn (Bin Arrow Unknown Unknown) Unknown (Lam (dyn_emb e))
     | dyn_lang.definition.App ℓ e1 e2 =>
-        App (Ascribe ℓ Unknown (Bin Arrow Unknown Unknown) (dyn_emb e1)) (dyn_emb e2)
+        App (Cast ℓ Unknown (Bin Arrow Unknown Unknown) (dyn_emb e1)) (dyn_emb e2)
     | dyn_lang.definition.InjL e =>
-        AscribeAn (Bin Sum Unknown Unknown) Unknown (InjL $ dyn_emb e)
+        CastAn (Bin Sum Unknown Unknown) Unknown (InjL $ dyn_emb e)
     | dyn_lang.definition.InjR e =>
-        AscribeAn (Bin Sum Unknown Unknown) Unknown (InjR $ dyn_emb e)
+        CastAn (Bin Sum Unknown Unknown) Unknown (InjR $ dyn_emb e)
     | dyn_lang.definition.Case ℓ e0 e1 e2 =>
-        Case (Ascribe ℓ Unknown (Bin Sum Unknown Unknown) (dyn_emb e0)) (dyn_emb e1) (dyn_emb e2)
+        Case (Cast ℓ Unknown (Bin Sum Unknown Unknown) (dyn_emb e0)) (dyn_emb e1) (dyn_emb e2)
     | dyn_lang.definition.Fst ℓ e =>
-        Fst (Ascribe ℓ Unknown (Bin Product Unknown Unknown) (dyn_emb e))
+        Fst (Cast ℓ Unknown (Bin Product Unknown Unknown) (dyn_emb e))
     | dyn_lang.definition.Snd ℓ e =>
-        Snd (Ascribe ℓ Unknown (Bin Product Unknown Unknown) (dyn_emb e))
+        Snd (Cast ℓ Unknown (Bin Product Unknown Unknown) (dyn_emb e))
     | dyn_lang.definition.Pair e1 e2 =>
-        AscribeAn (Bin Product Unknown Unknown) Unknown (Pair (dyn_emb e1) (dyn_emb e2))
-    | dyn_lang.definition.Error ℓ => Ascribe ℓ (Base Bool) Unknown (Ascribe ℓ Unknown (Base Bool)
-                                        (Ascribe ℓ (Base Unit) Unknown (Lit LitUnit)))
+        CastAn (Bin Product Unknown Unknown) Unknown (Pair (dyn_emb e1) (dyn_emb e2))
+    | dyn_lang.definition.Error ℓ => Cast ℓ (Base Bool) Unknown (Cast ℓ Unknown (Base Bool)
+                                        (Cast ℓ (Base Unit) Unknown (Lit LitUnit)))
     end.
 
   (* (at level 4, e at next level). *)
